Some experiments using new semantic types
Semantic types: type member introduction rule

theories/olty_experiments.v
@@ -110,3 +110,245 @@ Qed.
 End judgments.
 
 End OLty_judge.
+
+From D.Dot Require Import syn synLemmas rules typeExtractionSyn path_wp.
+
+Implicit Types
+         (v: vl) (e: tm) (d: dm) (ds: dms) (p : path).
+
+Module SemTypes.
+
+Include OLty syn.
+
+Class dlangG Σ := DLangG {
+  dlangG_savior :> savedInterpG Σ (var → vl) vl;
+  dlangG_interpNames :> gen_iheapG stamp gname Σ;
+}.
+
+Instance dlangG_irisG `{dlangG Σ} : irisG dlang_lang Σ := {
+  state_interp σ κs _ := True%I;
+  fork_post _ := True%I;
+}.
+
+Import mapsto.
+Notation "s ↝ φ" := (∃ γ, s ↦ γ ∗ γ ⤇ φ)%I  (at level 20) : bi_scope.
+
+Set Primitive Projections.
+Record dlty Σ := Dlty {
+  dlty_label : label;
+  dlty_car : ((var → vl) -d> dm -d> iProp Σ);
+  dlty_persistent ρ d :> Persistent (dlty_car ρ d);
+}.
+Global Arguments Dlty {_} _%I _ {_}.
+Global Arguments dlty_car {_} _ _ _ /.
+Global Arguments dlty_label {_} _ /.
+Global Existing Instance dlty_persistent.
+
+Section Judgments.
+  Context `{HdotG: dlangG Σ}.
+
+  Lemma leadsto_agree s (φ1 φ2 : infEnvD Σ) ρ v :
+    s ↝ φ1 -∗ s ↝ φ2 -∗ ▷ (φ1 ρ v ≡ φ2 ρ v).
+  Proof.
+    iIntros "/= #H1 #H2".
+    iDestruct "H1" as (γ1) "[Hs1 Hg1]".
+    iDestruct "H2" as (γ2) "[Hs2 Hg2]".
+    iDestruct (mapsto_agree with "Hs1 Hs2") as %->.
+    by iApply (saved_interp_agree _ φ1 φ2).
+  Qed.
+  Implicit Types (φ : olty Σ).
+
+  Definition interp_expr (φ : infEnvD Σ) :=
+    λ ρ t, WP t {{ φ ρ }} %I.
+  Global Arguments interp_expr /.
+
+  Definition ietp Γ φ e : iProp Σ := (⌜ nclosed e (length Γ) ⌝ ∗
+    □∀ ρ, ⟦Γ⟧* ρ → interp_expr φ (to_subst ρ) (e.|[to_subst ρ]))%I.
+  Global Arguments ietp /.
+
+  Definition step_indexed_ietp Γ φ e i: iProp Σ :=
+    (⌜ nclosed e (length Γ) ⌝ ∗ □∀ ρ, ⟦Γ⟧* ρ →
+      interp_expr (λ ρ v, ▷^i φ ρ v) (to_subst ρ) (e.|[to_subst ρ]))%I.
+  Global Arguments step_indexed_ietp /.
+
+  Definition step_indexed_ivstp Γ φ1 φ2 i j: iProp Σ :=
+    (□∀ ρ v, ⌜ nclosed_vl v 0 ⌝ →
+      ⟦Γ⟧*ρ → (▷^i φ1 (to_subst ρ) v) → ▷^j φ2 (to_subst ρ) v)%I.
+  Global Arguments step_indexed_ivstp /.
+
+  Definition idtp Γ l (T : dlty Σ) d : iProp Σ :=
+    (⌜ nclosed d (length Γ) ⌝ ∧ ⌜ l = dlty_label T ⌝ ∗
+      □∀ ρ, ⟦Γ⟧* ρ → dlty_car T (to_subst ρ) d.|[to_subst ρ])%I.
+
+  Global Arguments idtp /.
+End Judgments.
+
+Notation "Γ ⊨ e : φ" := (ietp Γ φ e) (at level 74, e, φ at next level).
+Notation "Γ ⊨ e : T , i" := (step_indexed_ietp Γ T e i) (at level 74, e, T at next level).
+Notation "Γ ⊨ [ φ1 , i ]  <: [ φ2 , j ]" := (step_indexed_ivstp Γ φ1 φ2 i j) (at level 74, φ1, φ2 at next level): bi_scope.
+Notation "Γ ⊨d{ l := d  } : T" := (idtp Γ l T d) (at level 64, d, l, T at next level).
+
+Section SemTypes.
+  Context `{HdotG: dlangG Σ}.
+
+  Implicit Types (φ: olty Σ) (τ : vl → iProp Σ).
+
+  Program Definition closed_olty (φ : infEnvD Σ) `{∀ ρ v, Persistent (φ ρ v)} : olty Σ :=
+    Olty (λ ρ v, ⌜ nclosed_vl v 0 ⌝ ∗ φ ρ v)%I _.
+  Next Obligation. iIntros (????) "[$_]". Qed.
+
+  Program Definition lift_dinterp_vl (T : dlty Σ): olty Σ :=
+    closed_olty (λ ρ v, (∃ d, ⌜v @ dlty_label T ↘ d⌝ ∧ dlty_car T ρ d)%I).
+
+  Definition oLater φ :=
+    closed_olty (λ ρ v, ▷ φ ρ v)%I.
+
+  (* Global Arguments sem_sel /. *)
+
+  Lemma iterate_TLater_later i (φ : olty Σ) ρ v:
+    nclosed_vl v 0 →
+    (iterate oLater i φ) ρ v ≡ (▷^i φ ρ v)%I.
+  Proof.
+    elim: i => [|i IHi] // => Hcl. rewrite iterate_S /= IHi //.
+    iSplit; by [iIntros "#[_ $]" | iIntros "$"].
+  Qed.
+
+  Definition idm_proj_semtype d τ : iProp Σ :=
+    (∃ s σ interp, ⌜ d = dtysem σ s ∧ τ = interp (to_subst σ) ⌝ ∗ s ↝ interp)%I.
+  Notation "d ↗ τ" := (idm_proj_semtype d τ) (at level 20).
+  Global Instance idm_proj_persistent d τ: Persistent (d ↗ τ) := _.
+
+  Lemma stored_pred_agree d τ1 τ2 v :
+    d ↗ τ1 -∗ d ↗ τ2 -∗ ▷ (τ1 v ≡ τ2 v).
+  Proof.
+    iIntros "/= #Hd1 #Hd2".
+    iDestruct "Hd2" as (s' σ' interp2 ?) "Hs2".
+    iDestruct "Hd1" as (s σ interp1 ?) "Hs1".
+    ev; simplify_eq. by iApply (leadsto_agree _ interp1 interp2).
+  Qed.
+
+  Lemma idm_proj_intro s σ (φ : infEnvD Σ) :
+    s ↝ φ -∗ dtysem σ s ↗ φ (to_subst σ).
+  Proof. iIntros. iExists s, σ , φ. by iSplit. Qed.
+
+  Global Opaque idm_proj_semtype.
+
+  Definition oDTMem l φ1 φ2 : dlty Σ := Dlty l
+    (λ ρ d,
+    ∃ τ, (d ↗ τ) ∗
+       □ ((∀ v, ⌜ nclosed_vl v 0 ⌝ → ▷ φ1 ρ v → □ ▷ τ v) ∗
+          (∀ v, ⌜ nclosed_vl v 0 ⌝ → □ ▷ τ v → ▷ φ2 ρ v)))%I.
+
+  Definition oTTMem l φ1 φ2 :=
+    lift_dinterp_vl (oDTMem l φ1 φ2).
+
+  Definition oDVMem l φ : dlty Σ := Dlty l
+    (λ ρ d, ∃ vmem, ⌜d = dvl vmem⌝ ∧ ▷ φ ρ vmem)%I.
+
+  Definition oTVMem l φ :=
+    lift_dinterp_vl (oDVMem l φ).
+
+  Definition infEnvD_equiv n (φ1 φ2 : infEnvD Σ) : iProp Σ :=
+    (∀ ρ v, ⌜ nclosed_sub n 0 ρ ⌝ → φ1 ρ v ≡ φ2 ρ v)%I.
+  Notation "φ1 ≈[  n  ] φ2" := (infEnvD_equiv n φ1 φ2) (at level 70).
+
+  Definition leadsto_infEnvD_equiv (sσ: extractedTy) n (φ : infEnvD Σ) : iProp Σ :=
+    let '(s, σ) := sσ in
+    (⌜nclosed_σ σ n⌝ ∧ ∃ (φ' : infEnvD Σ), s ↝ φ' ∗
+      infEnvD_equiv n φ (λ ρ, φ' (to_subst σ.|[ρ])))%I.
+  Notation "sσ ↝[  n  ] φ" := (leadsto_infEnvD_equiv sσ n φ) (at level 20).
+
+  Lemma D_Typ Γ T L U s σ l :
+    Γ ⊨ [T, 1] <: [U, 1] -∗
+    Γ ⊨ [L, 1] <: [T, 1] -∗
+    (s, σ) ↝[ length Γ ] T -∗
+    Γ ⊨d{ l := dtysem σ s } : oDTMem l L U.
+  Proof.
+    iIntros "#HTU #HLT #[% Hs] /="; repeat iSplit; [auto using fv_dtysem..|].
+    iIntros "!>" (ρ) "#Hg /=".
+    iDestruct (env_oltyped_fin_cl_ρ with "Hg") as %Hclp.
+    iDestruct "Hs" as (φ) "[Hγ Hγφ]".
+    iExists (φ (to_subst σ.|[to_subst ρ])); iSplit.
+    by iApply idm_proj_intro.
+    iModIntro; repeat iSplitL; iIntros (v Hclv) "#HL".
+    - iIntros "!>". iApply (internal_eq_iff with "(Hγφ [#//])").
+      by iApply "HLT".
+    - iApply "HTU" => //.
+      by iApply (internal_eq_iff with "(Hγφ [#//])").
+  Qed.
+
+  Lemma D_Typ_Concr Γ φ s σ l:
+    (s, σ) ↝[ length Γ ] φ -∗
+    Γ ⊨d{ l := dtysem σ s } : oDTMem l φ φ.
+  Proof. iIntros "#Hs"; iApply D_Typ; by [| iIntros "!> **"]. Qed.
+(*
+  Program Definition oInterp T := Olty ⟦ T ⟧ _.
+  Next Obligation. rewrite /vclosed=>*. by rewrite interp_v_closed. Qed. *)
+
+  Definition oTSel p (l : label) :=
+    closed_olty (λ ρ v, path_wp p.|[ρ]
+      (λ vp, ∃ ϕ d, ⌜vp @ l ↘ d⌝ ∧ d ↗ ϕ ∧ □ ▷ ϕ v)%I).
+
+  Lemma Sub_Sel Γ L U va l i:
+    Γ ⊨ tv va : oTTMem l L U, i -∗
+    Γ ⊨ [oLater L, i] <: [oTSel (pv va) l, i].
+  Proof.
+    iIntros "#[% #Hva] !>" (ρ v Hclv) "#Hg #[_ HvL]". iFrame (Hclv).
+    iSpecialize ("Hva" with "Hg"). rewrite /= wp_value_inv'.
+    iNext.
+    iDestruct "Hva" as (Hclvas' d Hl φ) "#[Hlφ [#HLφ #HφU]]".
+    iExists φ, d; repeat iSplit => //. by iApply "HLφ".
+  Qed.
+
+  Lemma Sel_Sub Γ L U va l i:
+    Γ ⊨ tv va : oTTMem l L U, i -∗
+    Γ ⊨ [oTSel (pv va) l, i] <: [oLater U, i].
+  Proof.
+    iIntros "#[% #Hva] !>" (ρ v Hclv) "#Hg [$ #Hφ]". move: H => Hclva.
+    iSpecialize ("Hva" with "Hg"); rewrite /= wp_value_inv'.
+    iNext.
+    iDestruct "Hva" as (Hclvas d Hl φ) "#[Hlφ [#HLφ #HφU]]".
+    iDestruct "Hφ" as (φ1 d1 Hva) "[Hγ #HΦ1v]".
+    objLookupDet; subst. iDestruct (stored_pred_agree d _ _ v with "Hlφ Hγ") as "#Hag".
+    iApply "HφU" => //. iModIntro. iNext. by iRewrite "Hag".
+  Qed.
+
+(*
+  (* Alternative (and failed) definition. *)
+  Program Definition sem_sel p (l : label) :=
+    closed_olty (λ ρ v, path_wp p.|[ρ]
+      (λ vp, ∃ ϕ d, ⌜vp @ l ↘ d⌝ ∧ d ↗ ϕ ∧ □ ϕ v)%I).
+
+  Lemma Sub_Sel2 Γ L U va l i:
+    Γ ⊨ tv va : oTTMem l L U, i -∗
+    Γ ⊨ [oLater L, i] <: [oLater (sem_sel (pv va) l), i].
+  Proof.
+    iIntros "/= #[% #Hva] !>" (ρ v Hclv) "#Hg #[_ HvL]". move: H => Hclva. iFrame (Hclv).
+    iSpecialize ("Hva" with "Hg"); rewrite wp_value_inv'.
+    iNext.
+
+    iDestruct "Hva" as (Hclvas' d Hl φ) "#[Hlφ [#HLφ ?]]".
+    iSpecialize ("HLφ" $! _ Hclv with "HvL").
+    rewrite -later_intuitionistically.
+    iExists φ, d; by repeat iSplit.
+  Qed.
+
+  Lemma Sel_Sub2_Failed Γ L U va l i:
+    Γ ⊨ tv va : oTTMem l L U, i -∗
+    Γ ⊨ [oLater ((sem_sel (pv va) l)), i] <: [oLater U, i].
+  Proof.
+    iIntros "/= #[% #Hva] !>" (ρ v Hclv) "#Hg #[$ #[_ Hφ]]".
+    iSpecialize ("Hva" with "Hg"); rewrite wp_value_inv'.
+    iNext.
+    iDestruct "Hva" as (Hclvas d Hl φ) "#[Hlφ [_ #HφU]]".
+    iApply "HφU" => //.
+    rewrite -later_intuitionistically.
+    iDestruct "Hφ" as (φ1 d1) "[>% [Hγ #HΦ1v]]".
+    (* iSpecialize ("HLφ" $! v Hclv); iSpecialize ("HφU" $! v Hclv). *)
+    (* rewrite /sem_sel /olty_car. *)
+    objLookupDet; subst. iNext. iDestruct (stored_pred_agree d _ _ v with "Hlφ Hγ") as "#Hag".
+    repeat iModIntro. Fail by iRewrite "Hag".
+  Abort. *)
+
+End SemTypes.
+End SemTypes.
